\documentclass{article}

% Packages
\usepackage[a4paper,margin=3cm]{geometry}
\usepackage{amsmath}

% Commands
\renewcommand{\vec}{\mathbf}
\newcommand{\mat}{\mathbf}
\renewcommand{\d}{\partial}
\renewcommand{\min}{\mathrm{min}}
\renewcommand{\max}{\mathrm{max}}

% Document setup
\title{Ray Intersections With Depth Maps}
\author{Julian Bohnenk√§mper}

\begin{document}
\maketitle

\section{Basics}
View ray position $ \vec{v} = [v_x, v_y, v_z]^\top $ with direction $ \vec{w} = [w_x, w_y, w_z]^\top $.
The corresponding ray equation is:
$$
    \vec{v} + a \vec{w}
$$

The original camera is $ h $ unity away from the origin.

The following equation is for a ray from a pixel along the depth towards the camera.
\begin{align*}
    & \begin{bmatrix}
        x \\
        y \\
        0
    \end{bmatrix}
    +
    \frac{b}{h}
    \Bigg(
        \begin{bmatrix}
            0 \\
            0 \\
            h
        \end{bmatrix}
        -
        \begin{bmatrix}
            x \\
            y \\
            0
        \end{bmatrix}
    \Bigg)\\
    = & \begin{bmatrix}
        x \\
        y \\
        0
    \end{bmatrix}
    +
    \frac{b}{h}
    \begin{bmatrix}
        -x \\
        -y \\
        h
    \end{bmatrix}\\
    = & \begin{bmatrix}
        x \\
        y \\
        0
    \end{bmatrix}
    +
    b
    \begin{bmatrix}
        -x/h \\
        -y/h \\
        1
    \end{bmatrix}
\end{align*}

Now we need to find for which $x$'s and $y$'s an intersection with the view ray exists.

\begin{align*}
    & \vec{v} + a \vec{w} = \begin{bmatrix}
        x \\
        y \\
        0
    \end{bmatrix}
    +
    b
    \begin{bmatrix}
        -x/h \\
        -y/h \\
        1
    \end{bmatrix}\\
    \iff & \begin{cases}
        v_x + a \cdot w_x = x - \frac{b}{h} \cdot x \\
        v_y + a \cdot w_y = y - \frac{b}{h} \cdot y \\
        v_z + a \cdot w_z = b
    \end{cases}\\
    \iff & \begin{cases}
        v_x + a \cdot w_x = (1 - \frac{b}{h}) \cdot x \\
        v_y + a \cdot w_y = (1 - \frac{b}{h}) \cdot y \\
        v_z + a \cdot w_z = b
    \end{cases}\\
    \iff & \begin{cases}
        \frac{v_x + a \cdot w_x}{1 - b/h} = x \\
        \frac{v_y + a \cdot w_y}{1 - b/h} = y \\
        v_z + a \cdot w_z = b
    \end{cases}\\
    \implies & \begin{cases}
        \frac{v_x + a \cdot w_x}{1 - (v_z + a \cdot w_z)/h} = x \\
        \frac{v_y + a \cdot w_y}{1 - (v_z + a \cdot w_z)/h} = y
    \end{cases}\\
    \iff & \frac{1}{1 - (v_z + a \cdot w_z)/h}
    \bigg(
        \begin{bmatrix}
            v_x \\
            v_y
        \end{bmatrix}
        +
        a
        \begin{bmatrix}
            w_x \\
            w_y
        \end{bmatrix}
    \bigg)
    =
    \begin{bmatrix}
        x \\
        y
    \end{bmatrix}\\
    \iff & \frac{\vec{v}_{x,y} + a \cdot \vec{w}_{x,y}}{1 - (v_z + a \cdot w_z)/h} = [x, y]^\top
\end{align*}

Derivatives might be useful:
\begin{align*}
    \frac{\d [x, y]^\top}{\d a} &= \frac{\d}{\d a} \frac{\vec{v}_{x,y} + a \cdot \vec{w}_{x,y}}{1 - (v_z + a \cdot w_z)/h} \\
    &= \frac{\vec{w}_{x,y}}{1 - (v_z + a \cdot w_z)/h} + (\vec{v}_{x,y} + a \cdot \vec{w}_{x,y}) \cdot \frac{\d}{\d a} \frac{1}{1 - (v_z + a \cdot w_z)/h} \\
    &= \frac{\vec{w}_{x,y}}{1 - (v_z + a \cdot w_z)/h} + (\vec{v}_{x,y} + a \cdot \vec{w}_{x,y}) \cdot \frac{1}{(1 - (v_z + a \cdot w_z)/h)^2} \cdot \frac{\d}{\d a} \Big(1 - \frac{v_z + a \cdot w_z}{h}\Big)\\
    &= \frac{\vec{w}_{x,y}}{1 - (v_z + a \cdot w_z)/h} + \frac{\vec{v}_{x,y} + a \cdot \vec{w}_{x,y}}{(1 - (v_z + a \cdot w_z)/h)^2} \cdot \frac{w_z}{h}\\
    &= \frac{1}{1 - (v_z + a \cdot w_z)/h} \cdot \Big( \vec{w}_{x,y} + \frac{\vec{v}_{x,y} + a \cdot \vec{w}_{x,y}}{1 - (v_z + a \cdot w_z)/h} \cdot \frac{w_z}{h} \Big)\\
    &= c(a) \cdot \Big( \vec{w}_{x,y} + (\vec{v}_{x,y} + a \cdot \vec{w}_{x,y}) \cdot \frac{w_z \cdot c(a)}{h} \Big)\\
    &= c(a) \cdot \Big( \vec{w}_{x,y} + \frac{w_z \cdot c(a)}{h} \cdot \vec{v}_{x,y} + a \cdot \frac{w_z \cdot c(a)}{h} \cdot \vec{w}_{x,y} \Big)\\
    &= c(a) \cdot \Big( \frac{w_z \cdot c(a)}{h} \cdot \vec{v}_{x,y} + \Big(1 + a \cdot \frac{w_z \cdot c(a)}{h} \Big) \cdot \vec{w}_{x,y} \Big)\\
\end{align*}
Eh, this derivative is not super pretty (maybe it can be simplified, but I feel like this won't be used anyways).

Another useful thingo could be a start and end point for $a$. These are easy to find with this equation:
$$ v_z + a \cdot w_z = b. $$

Simply use the bounds of $b$ which we denote as $b_\min$ and $b_\max$ and solve for the corresponding $a_\min$ and $a_\max$:
$$ a_\min = \frac{b_\max - v_z}{w_z} \text{ and } a_\max = \frac{b_\min - v_z}{w_z} $$
Remember, min and max are reversed for $a$ and $b$ because $\vec{w}$ usually points in a negative direction.

Another useful thing we can do is solve for $a$ to get a specific $x$ or $y$ coordinate:
\begin{align*}
         & \frac{v_x + w_x \cdot a}{1 - (v_z + w_z \cdot a)/h} = x \\
    \iff & v_x + w_x \cdot a = \Big(1 - \frac{v_z + w_z \cdot a}{h} \Big) \cdot x \\
    \iff & v_x + w_x \cdot a = x - \frac{v_z \cdot x}{h} + \frac{w_z \cdot x}{h} \cdot a \\
    \iff & w_x \cdot a - \frac{w_z \cdot x }{h} \cdot a = x - \frac{v_z \cdot x}{h} - v_x \\
    \iff & \Big( w_x - \frac{w_z \cdot x }{h} \Big) \cdot a = x - \frac{v_z \cdot x}{h} - v_x \\
    \iff & a = \frac{x - \frac{v_z \cdot x}{h} - v_x}{w_x - \frac{w_z \cdot x}{h}} \\
    \iff & a = \frac{x - \Big( v_x - \frac{v_z \cdot x}{h} \Big)}{w_x - \frac{w_z \cdot x}{h}} \\
\end{align*}
TODO: Find a nicer way to write this (my guess is, that this can be a bit prettier)

\begin{align*}
    % & \frac{v_x + w_x \cdot (a_0 + \Delta a)}{1 - (v_z + w_z \cdot (a_0 + \Delta a))/h} = x_0 + \Delta x \\
    % \iff & \frac{v_x + w_x \cdot (a_0 + \Delta a)}{1 - (v_z + w_z \cdot (a_0 + \Delta a))/h} = x_0 + \Delta x \\
         & a_0 + \Delta a = \frac{(x_0 + \Delta x) - ( v_x - \frac{v_z \cdot (x_0 + \Delta x)}{h} )}{w_x - \frac{w_z \cdot (x_0 + \Delta x)}{h}} \\
    \iff & \frac{x_0 - ( v_x - \frac{v_z \cdot x_0}{h} )}{w_x - \frac{w_z \cdot x_0}{h}} + \Delta a = \frac{(x_0 + \Delta x) - ( v_x - \frac{v_z \cdot (x_0 + \Delta x)}{h} )}{w_x - \frac{w_z \cdot (x_0 + \Delta x)}{h}} \\
    \iff & \Delta a = \frac{(x_0 + \Delta x) - ( v_x - \frac{v_z \cdot (x_0 + \Delta x)}{h} )}{w_x - \frac{w_z \cdot (x_0 + \Delta x)}{h}} - \frac{x_0 - ( v_x - \frac{v_z \cdot x_0}{h} )}{w_x - \frac{w_z \cdot x_0}{h}} \\
    \iff & \Delta a = \frac{(x_0 + \Delta x) - ( v_x - \frac{v_z \cdot (x_0 + \Delta x)}{h} )}{w_x - \frac{w_z \cdot (x_0 + \Delta x)}{h}} \cdot \frac{w_x - \frac{w_z \cdot x_0}{h}}{w_x - \frac{w_z \cdot x_0}{h}} - \frac{x_0 - ( v_x - \frac{v_z \cdot x_0}{h} )}{w_x - \frac{w_z \cdot x_0}{h}} \cdot \frac{w_x - \frac{w_z \cdot (x_0 + \Delta x)}{h}}{w_x - \frac{w_z \cdot (x_0 + \Delta x)}{h}} \\
    \iff & \Delta a = \frac{(x_0 + \Delta x)(w_x - \frac{w_z \cdot x_0}{h}) - ( v_x - \frac{v_z \cdot (x_0 + \Delta x)}{h} )(w_x - \frac{w_z \cdot x_0}{h})}{( w_x - \frac{w_z \cdot (x_0 + \Delta x)}{h} ) (w_x - \frac{w_z \cdot x_0}{h})} \\
         &- \frac{x_0 (w_x - \frac{w_z \cdot (x_0 + \Delta x)}{h}) - ( v_x - \frac{v_z \cdot x_0}{h} ) (w_x - \frac{w_z \cdot (x_0 + \Delta x)}{h})}{(w_x - \frac{w_z \cdot x_0}{h})(w_x - \frac{w_z \cdot (x_0 + \Delta x)}{h})} \\
    \iff & \Delta a = \frac{1}{(w_x - \frac{w_z \cdot x_0}{h})(w_x - \frac{w_z \cdot (x_0 + \Delta x)}{h})} \\ 
         &\cdot ((x_0 + \Delta x)(w_x - \frac{w_z \cdot x_0}{h}) - ( v_x - \frac{v_z \cdot (x_0 + \Delta x)}{h} )(w_x - \frac{w_z \cdot x_0}{h}) \\
         &- (x_0 (w_x - \frac{w_z \cdot (x_0 + \Delta x)}{h}) - ( v_x - \frac{v_z \cdot x_0}{h} ) (w_x - \frac{w_z \cdot (x_0 + \Delta x)}{h}))) \\
    \iff & \Delta a = \frac{1}{(w_x - \frac{w_z \cdot x_0}{h})(w_x - \frac{w_z \cdot (x_0 + \Delta x)}{h})} \\ 
         &\cdot ((x_0 + \Delta x)(w_x - \frac{w_z \cdot x_0}{h}) - ( v_x - \frac{v_z \cdot (x_0 + \Delta x)}{h} )(w_x - \frac{w_z \cdot x_0}{h}) \\
         &- (x_0 (w_x - \frac{w_z \cdot (x_0 + \Delta x)}{h}) - ( v_x - \frac{v_z \cdot x_0}{h} ) (w_x - \frac{w_z \cdot (x_0 + \Delta x)}{h}))) \\
\end{align*}

$$
\frac{\Delta x - v_{x} + x_{0} + \frac{v_{z} \left(\Delta x + x_{0}\right)}{h}}{w_{x} - \frac{w_{z} \left(\Delta x + x_{0}\right)}{h}} - \frac{- v_{x} + x_{0} + \frac{v_{z} x_{0}}{h}}{w_{x} - \frac{w_{z} x_{0}}{h}}
$$
$$
\frac{\Delta x \cdot h \left(h w_{x} - v_{x} w_{z} + v_{z} w_{x}\right)}{- \Delta x \cdot h w_{x} w_{z} + \Delta x w_{z}^{2} x_{0} + h^{2} w_{x}^{2} - 2 h w_{x} w_{z} x_{0} + w_{z}^{2} x_{0}^{2}}
$$
$$
\Delta a = \frac{\Delta x h \left(h w_{x} - v_{x} w_{z} + v_{z} w_{x}\right)}{\left(h w_{x} - w_{z} x_{0}\right) \left(- \Delta x w_{z} + h w_{x} - w_{z} x_{0}\right)}
$$
This was "generated" with \texttt{sympy}.

\end{document}
